Current.thy
@@ -20,4 +20,8 @@ fun bottom :: "'a current \<Rightarrow> 'a current" where
 fun toList :: "'a current \<Rightarrow> 'a list" where
   "toList (Current extra _ old _) = extra @ (Stack.toList old)"
 
+fun isEmpty :: "'a current \<Rightarrow> bool" where
+  "isEmpty (Current [] _ old _) = Stack.isEmpty old"
+| "isEmpty _ = False"
+
 end
