Current_Proof.thy
@@ -1,9 +1,14 @@
 theory Current_Proof
-  imports Current
+  imports Current Stack_Proof
 begin
 
 lemma put: "toList (put x current) = x # Current.toList current"
   apply(induction x current rule: put.induct)
   by auto
+
+lemma get: "\<lbrakk>\<not> isEmpty current; get current = (x, current')\<rbrakk>
+  \<Longrightarrow> x # Current.toList current' = Current.toList current"
+  apply(induction current arbitrary: x rule: get.induct)
+  by(auto simp: first_pop)
 
 end
